sketch

SP1Chips/BitwiseChip.lean
@@ -5,58 +5,150 @@ open LeanRV32D.Functions Sail
 
 namespace BitwiseChip
 
-
 def constraints
-  (Main : Vector BabyBear 23)
-  : SP1ConstraintList :=
-  let E0 : BabyBear := Main[22] - 1
-  let E2 : BabyBear := Main[22] * E0
-  let E4 : BabyBear := Main[3] + 4
-  let E6 : BabyBear := 16384 * Main[1]
-  let E8 : BabyBear := E6 + Main[2]
-  [ .assertZero E2
-  ]
-  ++ (AddOperation.constraints #v[Main[11], Main[12], Main[16], Main[17], Main[20], Main[21], Main[22]])
-  ++ (CPUState.constraints
-      { shard := Main[0]
-      , clk_high_limb := Main[1]
-      , clk_low_limb := Main[2]
-      , pc := Main[3] }
-      E4
-      4
-      Main[22])
-  ++ (RTypeReader.constraints
+  (Main : Vector BabyBear 33)
+  : Word BabyBear × SP1ConstraintList :=
+  let Expr0 := Main[30] + Main[31]
+  let Expr2 := Expr0 + Main[32]
+  let Expr4 := Main[30] - 1
+  let Expr6 := Main[30] * Expr4
+  let Expr8 := Main[31] - 1
+  let Expr10 := Main[31] * Expr8
+  let Expr12 := Main[32] - 1
+  let Expr14 := Main[32] * Expr12
+  let Expr16 := Expr2 - 1
+  let Expr18 := Expr2 * Expr16
+  let Expr20 := Main[30] * 2
+  let Expr22 := Main[31] * 1
+  let Expr24 := Expr20 + Expr22
+  let Expr26 := Main[32] * 0
+  let Expr28 := Expr24 + Expr26
+  let Expr30 := Main[30] * 3
+  let Expr32 := Main[31] * 4
+  let Expr34 := Expr30 + Expr32
+  let Expr36 := Main[32] * 5
+  let Expr38 := Expr34 + Expr36
+  let Expr42 := Main[3] + 4
+  let Expr44 := 16384 * Main[1]
+  let Expr46 := Expr44 + Main[2]
+  let ⟨⟨⟨[Expr40, Expr41]⟩, _⟩, BitwiseU16Operation_constraints⟩ :=
+    BitwiseU16Operation.constraintList
+      #v[Main[11], Main[12]]
+      #v[Main[17], Main[18]]
+      { a_low_bytes := { low_bytes := #v[Main[22], Main[23]] }
+        b_low_bytes := { low_bytes := #v[Main[24], Main[25]] }
+        bitwise_operation :=
+          { result := #v[Main[26], Main[27], Main[28], Main[29]] } }
+      Expr28
+      Expr2
+  let CPUState_constraints : SP1ConstraintList := CPUState.constraints
+    { shard := Main[0]
+      clk_high_limb := Main[1]
+      clk_low_limb := Main[2]
+      pc := Main[3] }
+    Expr42
+    4
+    Expr2
+  let ALUTypeReader_constraints : SP1ConstraintList := ALUTypeReader.constraints
     Main[0]
-    E8
-    -- Main[3]
-    -- 0
-    #v[Main[20], Main[21]]
+    Expr46
+    Main[3]
+    Expr38
+    #v[Expr40, Expr41]
     { op_a := Main[4]
-    , op_a_memory :=
-        { prev_value := #v[Main[5], Main[6]]
-        , access_timestamp :=
-            { prev_clk := Main[7]
-            , diff_low_limb := Main[8]
+      op_a_memory :=
+        { prev_value := #v[Main[5], Main[6]],
+          access_timestamp :=
+            { prev_clk := Main[7],
+              diff_low_limb := Main[8] } }
+      op_a_0 := Main[9],
+      op_b := Main[10],
+      op_b_memory :=
+        { prev_value := #v[Main[11], Main[12]],
+          access_timestamp :=
+            { prev_clk := Main[13],
+              diff_low_limb := Main[14] } }
+      op_c := #v[Main[15], Main[16]],
+      op_c_memory :=
+        {
+          prev_value := #v[Main[17], Main[18]],
+          access_timestamp :=
+            {
+            prev_clk := Main[19],
+            diff_low_limb := Main[20]
             }
         }
-    , op_a_0 := Main[9]
-    , op_b := Main[10]
-    , op_b_memory :=
-        { prev_value := #v[Main[11], Main[12]]
-        , access_timestamp :=
-            { prev_clk := Main[13]
-            , diff_low_limb := Main[14]
-            }
-        }
-    , op_c := Main[15]
-    , op_c_memory :=
-        { prev_value := #v[Main[16], Main[17]]
-        , access_timestamp :=
-            { prev_clk := Main[18]
-            , diff_low_limb := Main[19]
-            }
-        }
+      imm_c := Main[21]
     }
-    Main[22])
+    Expr2
+  ⟨#v[Expr40, Expr41],
+    [ .assertZero Expr16,
+      .assertZero Expr10,
+      .assertZero Expr14,
+      .assertZero Expr18, ]
+    ++ BitwiseU16Operation_constraints
+    ++ CPUState_constraints
+    ++ ALUTypeReader_constraints⟩
+
+/-- `is_real` for the op is the sum of the individual opcodes. -/
+def is_real (Main : Vector BabyBear 33) : BabyBear :=
+  Main[30] + Main[31] + Main[32]
+
+section and
+
+def Word.bitvec_of_babybear (w : Word BabyBear) : BitVec 32 :=
+  BitVec.ofNatLT ((w[0] + w[1] * 65536) % 2^32) (by omega)
+
+-- def output_bitvec (Main : Vector BabyBear 33)
+
+def sp1_bitwise
+    (Main : Vector BabyBear 33)
+    -- (cstrs : (constraints Main).allHold)
+    -- (h_is_real : Main[22] = 1)
+    (rd rs1 rs2 : regidx) :
+    SailM Unit := do
+  writeReg Register.nextPC (BitVec.addInt (← readReg Register.PC) 4)
+  let _rs1_value ← rX_bits rs1
+  let _rs2_value ← rX_bits rs2
+  let output : Word BabyBear := (constraints Main).1
+  wX_bits rd (Word.bitvec_of_babybear output)
+
+def spec_and (rd rs1 rs2 : regidx) : SailM Unit := do
+  writeReg Register.nextPC (BitVec.addInt (← readReg Register.PC) 4)
+  let _ ← execute_RTYPE rs2 rs1 rd rop.AND
+  pure ()
+
+def spec_or (rd rs1 rs2 : regidx) : SailM Unit := do
+  writeReg Register.nextPC (BitVec.addInt (← readReg Register.PC) 4)
+  let _ ← execute_RTYPE rs2 rs1 rd rop.AND
+  pure ()
+
+def spec_xor (rd rs1 rs2 : regidx) : SailM Unit := do
+  writeReg Register.nextPC (BitVec.addInt (← readReg Register.PC) 4)
+  let _ ← execute_RTYPE rs2 rs1 rd rop.AND
+  pure ()
+
+theorem sp1_bitwise_eq_spec_and
+    (Main : Vector BabyBear 33)
+    (rd rs1 rs2 : regidx)
+    (h_is_and : Main[30] = 1) :
+    sp1_bitwise Main rd rs1 rs2 = spec_and rd rs1 rs2 := by
+  sorry
+
+theorem sp1_bitwise_eq_spec_or
+    (Main : Vector BabyBear 33)
+    (rd rs1 rs2 : regidx)
+    (h_is_or : Main[31] = 1) :
+    sp1_bitwise Main rd rs1 rs2 = spec_or rd rs1 rs2 := by
+  sorry
+
+theorem sp1_bitwise_eq_spec_xor
+    (Main : Vector BabyBear 33)
+    (rd rs1 rs2 : regidx)
+    (h_is_xor : Main[32] = 1) :
+    sp1_bitwise Main rd rs1 rs2 = spec_xor rd rs1 rs2 := by
+  sorry
+
+end and
 
 end BitwiseChip
